More progress in spill simulation proof.

theories/Spilling/SpillSim.v
@@ -10,13 +10,6 @@ Section Correctness.
 
   Variable slot : var -> var.
 
-
-Instance SR : PointwiseProofRelationI (((set var) * (set var)) * params) := {
-   ParamRelIP RMZ Z Z' := Z' = slot_lift_params slot (fst RMZ) Z /\ Z = snd RMZ;
-   ArgRelIP V V' RMZ VL VL' :=
-     VL' = extend_args VL (mark_elements (snd RMZ) (fst (fst RMZ) ∩ snd (fst RMZ)))
-}.
-
 Smpl Add match goal with
          | [ |- context [ ❬@lookup_list ?X ?Y ?f ?L❭ ] ] =>
            rewrite (@lookup_list_length X Y f L)
@@ -319,7 +312,18 @@ Proof.
 Qed.
 
 
-Lemma agree_on_update_map X `{OrderedType X} Y `{OrderedType Y} (V:X->Y)
+Lemma agree_on_update_map X `{OrderedType X} Y `{OrderedType Y} (V:X->Y) (x:X) (v:Y)
+      (f:X->X) D `{Proper _ (_eq ==> _eq) f} `{Proper _ (_eq ==> _eq) V}
+  : injective_on {x; D} f
+    -> agree_on _eq D ((f ∘ V)[x <- v])  (fun y => V[f x <- v] (f y)).
+Proof.
+  intros Inj.
+  hnf; intros. lud; eauto.
+  - exfalso. rewrite H4 in *. eauto.
+  - exfalso. eapply Inj in e; eauto with cset.
+Qed.
+
+Lemma agree_on_update_list_map X `{OrderedType X} Y `{OrderedType Y} (V:X->Y)
       (L:list X) (L':list Y)
       (Len:❬L❭=❬L'❭) (f:X->X) D `{Proper _ (_eq ==> _eq) f} `{Proper _ (_eq ==> _eq) V}
   : injective_on (D ∪ of_list L) f
@@ -392,7 +396,7 @@ Proof.
   rewrite !lookup_list_map. rewrite map_map. rewrite <- !lookup_list_map.
   eapply lookup_list_agree. rewrite lookup_list_map.
   rewrite of_list_elements.
-  etransitivity; [| eapply agree_on_eq_oval, agree_on_update_map];
+  etransitivity; [| eapply agree_on_eq_oval, agree_on_update_list_map];
     [ | eauto with len | eapply proper_var | eapply proper_onv'
       | eapply injective_on_incl; eauto; rewrite <- VDincl, of_list_elements; clear; cset_tac ].
   rewrite (set_decomp Sp).
@@ -408,16 +412,18 @@ Proof.
     rewrite of_list_elements. hnf; intros; cset_tac.
 Qed.
 
-Lemma regs_untouched_after_spill_load (V V':var->option val) VD R M K Sp L0
+Lemma regs_untouched_after_spill_load (V V' V'':var->option val) VD R M K Sp L0
+      (Agr3 : agree_on eq (R ∪ map slot M ∪ map slot Sp ∪ L0)
+                       (V' [slot ⊝ elements Sp <-- V' ⊝ elements Sp]
+                           [elements L0 <-- V' [slot ⊝ elements Sp <-- V' ⊝ elements Sp]
+                                     ⊝ slot ⊝ elements L0]) V'')
       (Disj : disj VD (map slot VD)) (Incl : R ∪ M [<=] VD)
       (Agr1 : agree_on eq R V V')
       (VDincl:Sp ∪ L0 [<=] VD)
-  :  agree_on eq ((R \ K) \ L0) V
-              (V' [slot ⊝ elements Sp <-- V' ⊝ elements Sp]
-                  [elements L0 <-- V' [slot ⊝ elements Sp <-- V' ⊝ elements Sp]
-                            ⊝ slot ⊝ elements L0]).
+  :  agree_on eq ((R \ K) \ L0) V V''.
 Proof.
   etransitivity; [eapply agree_on_incl; [eapply Agr1| clear; cset_tac]|].
+  etransitivity; [|eapply agree_on_incl; [eapply Agr3| clear; cset_tac]].
   eapply agree_on_update_list_dead.
   eapply agree_on_update_list_dead. reflexivity.
   rewrite of_list_map, of_list_elements; eauto.
@@ -427,20 +433,23 @@ Proof.
   rewrite of_list_elements. clear; hnf; intros; cset_tac.
 Qed.
 
-Lemma regs_agree_after_spill_load (V V':var->option val) VD R M K Sp L0
+Lemma regs_agree_after_spill_load (V V' V'':var -> option val) VD R M K Sp L0
+      (Agr3 : agree_on eq (R ∪ map slot M ∪ map slot Sp ∪ L0)
+                       (V' [slot ⊝ elements Sp <-- V' ⊝ elements Sp]
+                           [elements L0 <-- V' [slot ⊝ elements Sp <-- V' ⊝ elements Sp]
+                                     ⊝ slot ⊝ elements L0]) V'')
       (Inj : injective_on VD slot) (Disj : disj VD (map slot VD)) (Incl : R ∪ M [<=] VD)
       (Agr1 : agree_on eq R V V')
       (Agr2 : agree_on eq M V (fun x : var => V' (slot x)))
       (VDincl:Sp ∪ L0 [<=] VD) (SpR:Sp [<=] R) (LSpM:L0 [<=] Sp ∪ M)
-  : agree_on eq (R \ K ∪ L0) V
-             (V' [slot ⊝ elements Sp <-- V' ⊝ elements Sp]
-                 [elements L0 <-- V' [slot ⊝ elements Sp <-- V' ⊝ elements Sp]
-                           ⊝ slot ⊝ elements L0]).
+  : agree_on eq (R \ K ∪ L0) V V''.
 Proof.
+  etransitivity; [|eapply agree_on_incl; [eapply Agr3| clear; cset_tac]].
   rewrite union_comm, union_exclusive.
   eapply agree_on_union.
   -- eapply load_agree_after_spill_load; eauto.
   -- eapply regs_untouched_after_spill_load; eauto.
+     reflexivity.
 Qed.
 
 
@@ -457,12 +466,17 @@ Qed.
 
 Lemma agree_on_comp_both X `{OrderedType X} Y
       (V V':X->Y) (f:X->X) D `{Proper _ (_eq ==> _eq) f}
+      `{Proper _ (_eq ==> eq) V}
+      `{Proper _ (_eq ==> eq) V'}
   : agree_on eq (map f D) V V'
-    -> agree_on eq D (fun x => V (f x)) (fun x => V' (f x)).
+    <-> agree_on eq D (fun x => V (f x)) (fun x => V' (f x)).
 Proof.
-  intros.
-  hnf; intros. rewrite H1; eauto.
-  eapply map_iff; eauto.
+  split; intros Agr; hnf; intros.
+  + rewrite Agr; eauto.
+    eapply map_iff; eauto.
+  + eapply map_iff in H3; eauto; dcr.
+    exploit (Agr x0); eauto.
+    rewrite <- H6 in H3. eauto.
 Qed.
 
 Lemma injective_disj X `{OrderedType X} s t (f:X->X) `{Proper _ (_eq ==> _eq) f}
@@ -491,7 +505,7 @@ Proof.
   eapply agree_on_comp; eauto; [ symmetry; eapply agree_on_incl; eauto with cset | ].
   etransitivity; [eapply agree_on_incl; [eapply Agr1| eauto with cset]|].
   eapply agree_on_update_list_dead_slot; eauto.
-  etransitivity; [| eapply agree_on_eq_oval, agree_on_update_map];
+  etransitivity; [| eapply agree_on_eq_oval, agree_on_update_list_map];
     [ | eauto with len | eapply proper_var | eapply proper_onv'
       | eapply injective_on_incl; eauto; rewrite <- VDincl, of_list_elements;
         clear; cset_tac ].
@@ -515,7 +529,7 @@ Lemma mem_untouched_after_spill_load (V V' V'':var->option val) VD R M Sp L0
   : agree_on eq (M \ Sp) V (fun x : var => V'' (slot x)).
 Proof.
   etransitivity; [eapply agree_on_incl; [eapply Agr2| eauto with cset ]|].
-  eapply agree_on_comp_both; eauto.
+  eapply agree_on_comp_both; eauto using proper_onv.
   etransitivity; [| eapply agree_on_incl; [eapply Agr3| eauto with cset]].
   eapply agree_on_update_list_dead.
   eapply agree_on_update_list_dead. reflexivity.
@@ -531,14 +545,14 @@ Proof.
 Qed.
 
 Lemma mem_agrees_after_spill_load (V V' V'':var->option val) VD R M Sp L0
-      (Inj : injective_on VD slot) (Disj : disj VD (map slot VD)) (Incl : R ∪ M [<=] VD)
-      (Agr1 : agree_on eq R V V')
-      (Agr2 : agree_on eq M V (fun x : var => V' (slot x)))
-      (VDincl:Sp ∪ L0 [<=] VD) (SpR:Sp [<=] R) (LSpM:L0 [<=] Sp ∪ M)
       (Agr3 : agree_on eq (R ∪ map slot M ∪ map slot Sp ∪ L0)
                        (V' [slot ⊝ elements Sp <-- V' ⊝ elements Sp]
                            [elements L0 <-- V' [slot ⊝ elements Sp <-- V' ⊝ elements Sp]
                                      ⊝ slot ⊝ elements L0]) V'')
+      (Inj : injective_on VD slot) (Disj : disj VD (map slot VD)) (Incl : R ∪ M [<=] VD)
+      (Agr1 : agree_on eq R V V')
+      (Agr2 : agree_on eq M V (fun x : var => V' (slot x)))
+      (VDincl:Sp ∪ L0 [<=] VD) (SpR:Sp [<=] R) (LSpM:L0 [<=] Sp ∪ M)
   : agree_on eq (Sp ∪ M) V (fun x : var => V'' (slot x)).
 Proof.
   rewrite union_exclusive.
@@ -547,25 +561,175 @@ Proof.
   -- eapply mem_untouched_after_spill_load; try eapply Agr3; eauto.
 Qed.
 
+Inductive defined X : list (option X) -> Prop :=
+| NilDefined : defined nil
+| ConsDefined x xs: defined xs -> defined (Some x::xs).
+
+Lemma defined_get X (L:list (option X)) n x
+  : defined L
+    -> get L n x
+    -> exists y, x = Some y.
+Proof.
+  intros. general induction H0; invt defined; eauto.
+Qed.
+
+Lemma defined_on_update_list' X `{OrderedType X} Y (E:X -> option Y) L L' (Len:❬L❭=❬L'❭) s
+  : defined_on (s \ of_list L) E
+    -> defined L'
+    -> defined_on s (E [L <-- L']).
+Proof.
+  intros.
+  hnf; intros. decide (x ∈ of_list L).
+  - edestruct update_with_list_lookup_in_list; try eapply i; dcr; eauto.
+    rewrite H6. exploit defined_get; eauto.
+  - rewrite lookup_set_update_not_in_Z; eauto.
+    eapply H0; cset_tac.
+Qed.
+
+Lemma get_defined X (L:list (option X))
+  : (forall n x, get L n x -> exists y, x = Some y)
+    -> defined L.
+Proof.
+  intros. general induction L; eauto using defined, get.
+  edestruct H; dcr; eauto using get. subst.
+  eauto using defined, get.
+Qed.
+
+Lemma defined_on_defined X `{OrderedType X} Y (V:X->option Y) L
+      `{Proper _ (_eq ==> eq) V}
+  : defined_on (of_list L) V
+    <-> defined (V ⊝ L).
+Proof.
+  split; intros.
+  - eapply get_defined; intros; inv_get.
+    eapply get_in_of_list in H2. eauto.
+  - hnf; intros.
+    edestruct of_list_get_first; eauto; dcr.
+    eapply defined_get; eauto.
+    rewrite H4. eapply map_get_1; eauto.
+Qed.
+
+Lemma defined_on_comp X `{OrderedType X} Y (f:X->X) D (V:X -> option Y)
+      `{Proper _ (_eq ==> _eq) f}  `{Proper _ (_eq ==> eq) V}
+  : defined_on (map f D) V <-> defined_on D (f ∘ V).
+Proof.
+  split; intros; hnf; intros.
+  - exploit H2; eauto. eapply map_iff; eauto.
+  - eapply map_iff in H3; dcr; eauto.
+    setoid_rewrite H6; eauto.
+Qed.
+
+Lemma agree_on_update_dead_both_comp_right X `{OrderedType X} Y R
+      (lv:set X) (E E':X -> Y) (f:X->X) `{Proper _ (_eq ==> _eq) f} x v v'
+  : ~x ∈ lv
+    -> disj {x; lv} (map f lv)
+    -> agree_on R lv E (f ∘ E')
+    -> agree_on R lv (E [x <- v]) (f ∘ (E'[x <- v'])).
+Proof.
+  intros NotIn Disj Agr; unfold comp.
+  hnf; intros. lud; eauto.
+  exfalso. eapply (Disj x); eauto. cset_tac.
+  eapply map_iff; eauto.
+Qed.
+
+Lemma mem_agrees_after_spill_load_update (V V' V'':var->option val) VD R M Sp L0 x v
+      (Agr5 : agree_on eq (Sp ∪ M) V (fun x : var => V'' (slot x)))
+      (Disj : disj VD (map slot VD)) (Incl : R ∪ M [<=] VD) (NotIn: x ∉ Sp ∪ M)
+      (xIn:x ∈ VD)
+      (Agr1 : agree_on eq R V V')
+      (Agr2 : agree_on eq M V (fun x : var => V' (slot x)))
+      (VDincl:Sp ∪ L0 [<=] VD) (SpR:Sp [<=] R) (LSpM:L0 [<=] Sp ∪ M)
+      (Agr3 : agree_on eq (R ∪ map slot M ∪ map slot Sp ∪ L0)
+                       (V' [slot ⊝ elements Sp <-- V' ⊝ elements Sp]
+                           [elements L0 <-- V' [slot ⊝ elements Sp <-- V' ⊝ elements Sp]
+                                     ⊝ slot ⊝ elements L0]) V'')
+  : agree_on eq (Sp ∪ M) (V [x <- ⎣ v ⎦]) (fun x0 : var => (V'' [x <- ⎣ v ⎦]) (slot x0)).
+Proof.
+  eapply agree_on_update_dead_both_comp_right; eauto.
+  eapply disj_1_incl. eapply disj_2_incl; eauto.
+  eapply map_incl; eauto. rewrite <- Incl, SpR; reflexivity.
+  rewrite SpR, Incl. cset_tac.
+Qed.
+
+Lemma defined_on_after_spill_load (V V' V'':var->option val) VD R M Sp L0  K
+      (Agr5 : agree_on eq (Sp ∪ M) V (fun x : var => V'' (slot x)))
+      (Disj : disj VD (map slot VD)) (Incl : R ∪ M [<=] VD)
+      (Agr1 : agree_on eq R V V') (Def : defined_on (R ∪ map slot M) V')
+      (Agr2 : agree_on eq M V (fun x : var => V' (slot x)))
+      (VDincl:Sp ∪ L0 [<=] VD) (SpR:Sp [<=] R) (LSpM:L0 [<=] Sp ∪ M)
+      (Agr3 : agree_on eq (R ∪ map slot M ∪ map slot Sp ∪ L0)
+                       (V' [slot ⊝ elements Sp <-- V' ⊝ elements Sp]
+                           [elements L0 <-- V' [slot ⊝ elements Sp <-- V' ⊝ elements Sp]
+                                     ⊝ slot ⊝ elements L0]) V'')
+  : defined_on (R \ K ∪ L0 ∪ map slot (Sp ∪ M)) V''.
+Proof.
+  assert (defined_on Sp V') as DefSp by eauto using defined_on_incl with cset.
+  rewrite union_exclusive.
+  eapply defined_on_union.
+  -- eapply defined_on_agree_eq; [|eapply agree_on_incl;[eapply Agr3| eauto with cset]].
+     rewrite union_comm, union_exclusive. eapply defined_on_union.
+     ++ eapply defined_on_update_list'; eauto with len.
+       rewrite of_list_elements. clear; hnf; intros; cset_tac.
+       eapply defined_on_defined. clear; intuition.
+       rewrite of_list_map, of_list_elements; eauto.
+       eapply defined_on_update_list'; eauto with len.
+       rewrite of_list_map, of_list_elements; eauto.
+       rewrite LSpM. eapply (defined_on_incl Def); eauto.
+       rewrite map_union; eauto. clear; cset_tac.
+       eapply defined_on_defined. clear; intuition. eauto.
+       rewrite of_list_elements. eauto.
+     ++ eapply defined_on_agree_eq; [| eapply agree_on_update_list_dead; try reflexivity].
+       eapply defined_on_update_list'; eauto with len.
+       rewrite of_list_map, of_list_elements; eauto.
+       eapply (defined_on_incl Def). clear; cset_tac.
+       eapply defined_on_defined. clear; intuition. eauto.
+       rewrite of_list_elements. eauto.
+       rewrite of_list_elements. eauto. clear; hnf; intros; cset_tac.
+  -- rewrite map_union; eauto.
+     eapply defined_on_agree_eq; [ | eapply agree_on_incl; [ eapply Agr3| clear; cset_tac]];
+       eauto.
+     eapply defined_on_agree_eq; [| eapply agree_on_update_list_dead; try reflexivity].
+     eapply defined_on_update_list'; eauto with len.
+     rewrite of_list_map, of_list_elements; eauto.
+     eapply (defined_on_incl Def). clear; cset_tac.
+     eapply defined_on_defined. clear; intuition. eauto.
+     rewrite of_list_elements. eauto.
+     rewrite of_list_elements. clear; hnf; intros; cset_tac.
+Qed.
+
+
+Instance SR (VD:set var) : PointwiseProofRelationI (((set var) * (set var)) * params) := {
+   ParamRelIP RMZ Z Z' := Z' = slot_lift_params slot (fst RMZ) Z /\ Z = snd RMZ;
+   ArgRelIP V V' RMZ VL VL' :=
+     VL' = extend_args VL (mark_elements (snd RMZ) (fst (fst RMZ) ∩ snd (fst RMZ))) /\
+     agree_on eq (fst (fst RMZ)) V V' /\
+     agree_on eq (snd (fst RMZ)) V (fun x => V' (slot x)) /\
+     (fst (fst RMZ) ∪ snd (fst RMZ)) ⊆ VD
+}.
+
 
 Lemma sim_I k Λ ZL LV VD r L L' V V' R M s lv sl ib ra
   : agree_on eq R V V'
     -> agree_on eq M V (fun x => V' (slot x))
-  -> live_sound Imperative ZL LV s lv
-  -> spill_sound k ZL Λ (R,M) s sl
-  -> spill_live VD sl lv
-  -> injective_on VD slot
-  -> disj VD (map slot VD)
-  -> defined_on (R ∪ map slot M) V'
-  -> R ∪ M ⊆ VD
-  -> labenv_sim Sim (sim r) SR (zip pair Λ ZL) L L'
-  -> (fst (getAnn ra) ∪ snd (getAnn ra)) ⊆ VD
-  -> renamedApart s ra
-  -> sim r Sim (L, V, s) (L', V', do_spill slot s sl ib).
+    -> live_sound Imperative ZL LV s lv
+    -> spill_sound k ZL Λ (R,M) s sl
+    -> spill_live VD sl lv
+    -> injective_on VD slot
+    -> disj VD (map slot VD)
+    -> defined_on (R ∪ map slot M) V'
+    -> R ∪ M ⊆ fst (getAnn ra)
+    -> labenv_sim Sim (sim r) (SR VD) (zip pair Λ ZL) L L'
+    -> (fst (getAnn ra) ∪ snd (getAnn ra)) ⊆ VD
+    -> renamedApart s ra
+    -> sim r Sim (L, V, s) (L', V', do_spill slot s sl ib).
 Proof.
-  simpl. unfold reconstr_live_do_spill. unfold sim. revert_except s.
+  simpl. unfold reconstr_live_do_spill. unfold sim.
+  move VD before k. move s before VD. revert_until s.
   time (sind s).
-  intros ? ? ? ? ? ? ? ? ? ? ? ? ? ? ? ? Agr1 Agr2 LS SLS SL Inj Disj Def Incl LSim RAincl RA.
+  intros ? ? ? ? ? ? ? ? ? ? ? ? ? ? Agr1 Agr2 LS SLS SL Inj Disj Def Incl' LSim RAincl RA.
+  assert (Incl:R ∪ M [<=] VD). {
+    rewrite <- RAincl, <- Incl'. eauto with cset.
+  }
   exploit L_sub_SpM as LSpM; eauto.
   exploit Sp_sub_R as SpR; eauto.
   assert (VDincl:getSp sl ∪ getL sl [<=] VD). {
@@ -577,90 +741,88 @@ Proof.
   eapply defined_on_incl; eauto.
   rewrite SpR at 1. rewrite LSpM.
   rewrite map_union; eauto. clear; cset_tac.
-  intros ? Agr3.
-  time (destruct s; invt spill_sound; invt spill_live; invt live_sound; invt renamedApart).
-  - simpl in *. simpl. rewrite elements_empty; simpl.
-    destruct e.
+  rewrite !lookup_list_map. intros ? Agr3.
+  time (destruct s; invt spill_sound; invt spill_live; invt live_sound; invt renamedApart);
+    exploit regs_agree_after_spill_load as Agr4; eauto;
+      exploit mem_agrees_after_spill_load as Agr5; eauto;
+        simpl in *; rewrite !elements_empty; simpl.
+  - destruct e; simpl in *.
     + eapply (sim_let_op il_statetype_I); eauto.
-      * eapply op_eval_live; eauto. eapply Op.live_freeVars.
-        simpl in *. admit.
+      * symmetry; eapply op_eval_agree; eauto using agree_on_incl.
       * intros. left. eapply IH; eauto.
         -- eapply agree_on_update_same; eauto.
-           eapply agree_on_incl. instantiate (1:=R \ K ∪ L0).
-           etransitivity; [| eapply agree_on_incl; [eapply Agr3| clear; cset_tac]].
-           rewrite !lookup_list_map.
-           eapply regs_agree_after_spill_load; eauto.
+           eapply agree_on_incl; eauto.
            clear; cset_tac.
-        -- admit.
-        -- eapply defined_on_update_some. admit.
-        -- rewrite LSpM, SpR. assert (x ∈ VD).
-           rewrite <- RAincl, H17; clear; cset_tac.
-           revert H0 Incl. clear; cset_tac; eapply Incl; cset_tac.
+        -- eapply mem_agrees_after_spill_load_update; eauto.
+           rewrite SpR, Incl'; eauto.
+           rewrite H17 in RAincl.
+           revert RAincl; clear; cset_tac. eapply RAincl; cset_tac.
+        -- eapply defined_on_update_some.
+           eapply defined_on_incl.
+           eapply defined_on_after_spill_load; eauto.
+           clear; cset_tac.
+        -- pe_rewrite. rewrite LSpM, SpR, <- Incl'. clear; cset_tac.
         -- pe_rewrite. rewrite <- RAincl. rewrite H17. clear; cset_tac.
     + eapply (sim_let_call il_statetype_I); eauto.
-      * admit.
+      * symmetry; eapply omap_op_eval_agree; eauto using agree_on_incl.
       * intros. left. eapply IH; eauto.
         -- eapply agree_on_update_same; eauto.
-           eapply agree_on_incl. instantiate (1:=R \ K ∪ L0).
-           etransitivity; [| eapply agree_on_incl; [eapply Agr3| clear; cset_tac]].
-           rewrite !lookup_list_map.
-           eapply regs_agree_after_spill_load; eauto.
+           eapply agree_on_incl; eauto.
            clear; cset_tac.
-        -- admit.
+        -- eapply mem_agrees_after_spill_load_update; eauto.
+           rewrite SpR, Incl'; eauto.
+           rewrite H17 in RAincl.
+           revert RAincl; clear; cset_tac. eapply RAincl; cset_tac.
         -- eapply defined_on_update_some. admit.
-        -- rewrite LSpM, SpR. assert (x ∈ VD).
-           rewrite <- RAincl, H17; clear; cset_tac.
-           revert H Incl. clear; cset_tac; eapply Incl; cset_tac.
+        -- pe_rewrite. rewrite LSpM, SpR, <- Incl'. clear; cset_tac.
         -- pe_rewrite. rewrite <- RAincl. rewrite H17. clear; cset_tac.
-  - simpl in *. rewrite elements_empty; simpl.
+  - simpl in *.
     eapply (sim_cond il_statetype_I); eauto.
-    + eapply op_eval_live; eauto.
-      admit.
+    + symmetry; eapply op_eval_agree; eauto using agree_on_incl.
     + intros; left. eapply IH; eauto.
-      * etransitivity; [| eapply agree_on_incl; [eapply H1| clear; cset_tac]].
-        rewrite !lookup_list_map.
-        eapply regs_agree_after_spill_load; eauto.
-      * rewrite !lookup_list_map in H1.
-        eapply mem_agrees_after_spill_load; try eapply H1; eauto.
-      * admit.
-      * rewrite H10, H0. rewrite <- Incl. clear; cset_tac.
+      * eapply defined_on_after_spill_load; eauto.
+      * pe_rewrite. rewrite LSpM, SpR, <- Incl'. clear; cset_tac.
+      * pe_rewrite. rewrite <- RAincl, <- H9. clear; cset_tac.
     + intros; left. eapply IH; eauto.
-      * etransitivity; [| eapply agree_on_incl; [eapply H1| clear; cset_tac]].
-        rewrite !lookup_list_map.
-        eapply regs_agree_after_spill_load; eauto.
-      * rewrite !lookup_list_map in H1.
-        eapply mem_agrees_after_spill_load; try eapply H1; eauto.
-      * admit.
-      * rewrite H10, H0. rewrite <- Incl. clear; cset_tac.
-  - simpl in *. rewrite elements_empty; simpl.
-    eapply labenv_sim_app; eauto using zip_get.
+      * eapply defined_on_after_spill_load; eauto.
+      * pe_rewrite. rewrite LSpM, SpR, <- Incl'. clear; cset_tac.
+      * pe_rewrite. rewrite <- RAincl, <- H9. clear; cset_tac.
+  - eapply labenv_sim_app; eauto using zip_get.
     intros; simpl in *; dcr; subst.
     split; eauto; intros.
     admit.
-  - simpl in *. rewrite elements_empty; simpl.
-    pno_step. simpl.
-    erewrite <- op_eval_agree; [reflexivity| |reflexivity].
-    symmetry. admit.
-  - simpl in *. rewrite elements_empty; simpl.
-    eapply sim_fun_ptw; eauto.
+  - pno_step. simpl.
+    erewrite op_eval_agree; [reflexivity| |reflexivity]. symmetry.
+    eapply agree_on_incl; eauto using regs_agree_after_spill_load; eauto.
+  - eapply sim_fun_ptw; try eapply LSim; eauto.
     + intros. left.
-      eapply IH; eauto using agree_on_incl.
-      * etransitivity; [| eapply agree_on_incl; [eapply H1| clear; cset_tac]].
-        rewrite !lookup_list_map.
-        eapply regs_agree_after_spill_load; eauto.
-      * rewrite !lookup_list_map in H1.
-        eapply mem_agrees_after_spill_load; try eapply H1; eauto.
-      * admit.
-      * rewrite H, H0. rewrite <- Incl. clear; cset_tac.
+      eapply (IH s); eauto using agree_on_incl.
+      * eapply defined_on_after_spill_load; eauto.
+      * pe_rewrite. rewrite LSpM, SpR, <- Incl'. clear; cset_tac.
+      * pe_rewrite. rewrite <- RAincl, <- H25. clear; cset_tac.
     + intros. hnf; intros; simpl in *; dcr. subst.
       inv_get. simpl.
-      exploit H23; eauto.
-      exploit H15; eauto.
-      exploit H18; eauto. destruct x.
-      exploit H17; eauto; simpl in *; dcr.
+      exploit H12; eauto.
+      exploit H20; eauto.
+      exploit H15; eauto. destruct x.
+      exploit H14; eauto; simpl in *; dcr.
+      exploit H2; eauto.
       exploit al_sub_RfMf; eauto.
       eapply IH; eauto.
-      admit. admit. admit. admit.
+      * admit.
+      * admit.
+      * admit.
+      * edestruct H8; eauto; dcr.
+        rewrite H39. simpl. simpl in *.
+        admit.
+      * edestruct H8; eauto; dcr.
+        rewrite H39. simpl. rewrite union_comm. rewrite <- union_assoc.
+        eapply union_incl_split.
+        -- rewrite <- RAincl. eapply incl_union_right.
+           rewrite <- H25. eapply incl_union_left.
+           eapply incl_list_union; eauto using zip_get.
+           unfold defVars. simpl. clear; eauto with cset.
+        -- rewrite <- RAincl. eauto with cset.
     + hnf; intros; simpl in *; subst.
       inv_get; simpl; eauto.
     + eauto with len.
